Fine/Completeness/SystemB.lean
@@ -1,0 +1,81 @@
+import Fine.Semantics.Model
+import Fine.Semantics.Satisfaction
+import Fine.Hilbert.SystemB
+import Fine.PropositionalLanguage
+
+def formalTheory (Γ : Ctx) : Prop := ∀f : Form, f ∈ Γ ↔ Γ ⊢ f
+
+def generatedTheory (Γ : Ctx) : Ctx := BProvable Γ
+
+prefix:512 "▲" => generatedTheory
+
+theorem generatedFormal : ∀Γ : Ctx, formalTheory (▲Γ) := by
+   unfold formalTheory
+   intros Γ f
+   apply Iff.intro
+   case mp =>
+      intros h₁
+      exact ⟨BProof.ax h₁, trivial⟩
+   case mpr =>
+      intros h₁
+      cases h₁; rename_i w _; induction w
+      case intro.ax => assumption
+      case intro.mp => 
+        rename_i _ P Q _ h₂ ih
+        have ⟨prf,_⟩ := ih
+        exact ⟨BProof.mp prf h₂, trivial⟩
+      case intro.adj => 
+        rename_i ih₁ ih₂
+        have ⟨prf₁,_⟩ := ih₁
+        have ⟨prf₂,_⟩ := ih₂
+        exact ⟨BProof.adj prf₁ prf₂, trivial⟩
+
+def DisjunctionClosed (Γ : Ctx) := ∀f g : Form, f ∈ Γ ∧ g ∈ Γ → f ¦ g ∈ Γ
+
+def PrimeTheory (Γ : Ctx) := ∀f g : Form, f ¦ g ∈ Γ → f ∈ Γ ∨ g ∈ Γ
+
+def FormalApplication (Γ : Ctx) (Δ : Ctx) : Ctx := 
+  λf : Form => ∃g : Form, g ∈ Δ ∧ (g ⊃ f) ∈ Γ
+
+def FormalDual (Γ : Ctx) : Ctx := 
+  λf : Form => ¬(~f ∈ Γ)
+
+lemma generatedDisjunction {f g h: Form} : f ∈ ▲{g} ∧ f ∈ ▲{h} → f ∈ ▲{g ¦ h} := by
+  intros h₁
+  have ⟨⟨prf₁,_⟩,prf₂,_⟩ := h₁
+  have l₁ := BTheorem.fromProof prf₁
+  have l₂ := BTheorem.fromProof prf₂
+  have l₃ := (BTheorem.mp (BTheorem.adj l₁ l₂) BTheorem.orE)
+  exact ⟨BTheorem.toProof l₃, trivial⟩
+
+lemma formalFixed {Γ : Ctx} : formalTheory Γ → ▲Γ = Γ := by
+  intros h₁
+  funext
+  case h x =>
+    ext
+    apply Iff.intro
+    case a.mp => 
+      intros a
+      exact (h₁ x).mpr a
+    case a.mpr =>
+      intros a
+      exact (h₁ x).mp a
+
+lemma BisFormal : formalTheory BTheory := by
+  unfold formalTheory
+  intros f
+  apply Iff.intro
+  case mp => intro a; exact ⟨BProof.ax a, trivial⟩
+  case mpr =>
+    intro h₁
+    have ⟨prf₁,_⟩ := h₁
+    induction prf₁
+    case ax _ P ih => assumption
+    case mp _ P Q prf₁ thm₁ ih => 
+      have l₁ := ih ⟨prf₁,trivial⟩
+      have ⟨thm₂,_⟩ := l₁
+      exact ⟨BTheorem.mp thm₂ thm₁, trivial⟩
+    case adj _ P Q prf₁ prf₂ ih₁ ih₂ =>
+      have ⟨l₁,_⟩ := ih₁ ⟨prf₁,trivial⟩
+      have ⟨l₂,_⟩ := ih₂ ⟨prf₂,trivial⟩
+      exact ⟨BTheorem.adj l₁ l₂, trivial⟩
